@prefix xsd: <http://www.w3.org/2001/XMLSchema#> .
@prefix rdf: <http://www.w3.org/1999/02/22-rdf-syntax-ns#> .
@prefix rdfs: <http://www.w3.org/2000/01/rdf-schema#> .
@prefix owl: <http://www.w3.org/2002/07/owl#> .
@prefix mismo: <http://www.mismo.org/residential/2009/schemas#> .


# Collection classes (Pattern 007) - using owl:Class
mismo:ABOUT_VERSIONS a owl:Class ;
    rdfs:label "About Versions Collection" ;
    rdfs:comment "Information about one or more ABOUT_VERSION. Holds all occurrences of ABOUT_VERSION." ;
    rdfs:subClassOf owl:Thing .

# Element classes (Pattern 006) - using owl:Class
mismo:ABOUT_VERSION a owl:Class ;
    rdfs:label "About Version" ;
    rdfs:comment "Information that identifies the version of the specification, software and/or data used for this transaction." ;
    rdfs:subClassOf mismo:ABOUT_VERSIONS .

# Object properties for containment
mismo:containsABOUT_VERSION a owl:ObjectProperty ;
    rdfs:label "contains ABOUT_VERSION" ;
    rdfs:comment "Relates ABOUT_VERSIONS to individual ABOUT_VERSION instances" ;
    owl:domain mismo:ABOUT_VERSIONS ;
    owl:range mismo:ABOUT_VERSION ;
    rdfs:subPropertyOf rdf:member .